Define S and D matrices, lemma for S correctness
Include prop for term being sematically equal to c(al)

proofs/core/PatternProofs.v
@@ -1,12 +1,16 @@
 Require Import Pattern.
 Require Import Denotational.
 
-(*First, we define the semantics of multiple pattern matching*)
-Section MultipleMatchSemantics.
+Section PatProofs.
+
 Context {gamma: context} (gamma_valid: valid_context gamma).
 Context (pd: pi_dom) (pf: pi_funpred gamma_valid pd) (vt: val_typevar).
+Variable (v: val_vars pd vt).
 Variable (b: bool). (*Generic over terms and formulas*)
 Variable (ret_ty : gen_type b). (*The return type of the values*)
+
+(*First, we define the semantics of multiple pattern matching*)
+Section MultipleMatchSemantics.
 
 (*Generalized term/formula rep*)
 Definition gen_rep (v: val_vars pd vt) (ty: gen_type b) (d: gen_term b) (Hty: gen_typed b d ty) : gen_ret pd vt b ty :=
@@ -59,17 +63,260 @@ Proof.
 Qed.
 
 (*Semantics for whole matrix matching*)
-Equations matches_matrix (v: val_vars pd vt) (tys: list vty) 
+Equations matches_matrix  (tys: list vty) 
   (al: arg_list (domain (dom_aux pd)) (map (v_subst vt) tys))
   (p: pat_matrix)
   (Hty: pat_matrix_typed tys p) :
   option (gen_ret pd vt b ret_ty):=
-matches_matrix v tys al nil Hty := None;
-matches_matrix v tys al (row :: ps) Hty :=
+matches_matrix tys al nil Hty := None;
+matches_matrix tys al (row :: ps) Hty :=
   match (matches_row tys al (fst row) (Forall_inv (proj1 Hty))) with
     | Some l => Some (gen_rep (extend_val_with_list pd vt v l) ret_ty (snd row) (Forall_inv (proj2 Hty)))
-    | None => matches_matrix v tys al ps (pat_matrix_typed_tail Hty)
+    | None => matches_matrix tys al ps (pat_matrix_typed_tail Hty)
   end.
+
+(*TODO (later): prove these equivalent to semantics in Denotational.v*)
+
+(*One more version, when we start with terms*)
+Equations terms_to_hlist (ts: list term) (tys: list vty)
+  (Hty: Forall2 (fun t ty => term_has_type gamma t ty) ts tys) :
+  arg_list (domain (dom_aux pd)) (map (v_subst vt) tys) :=
+terms_to_hlist nil nil Hty := HL_nil _;
+terms_to_hlist (t :: ts) (ty :: tys) Hty :=
+  HL_cons _ _ _ (term_rep gamma_valid pd vt pf v t ty (Forall2_inv_head Hty)) 
+    (terms_to_hlist ts tys (Forall2_inv_tail Hty)).
+  (*Wow equations is magic*)
+
+Definition matches_matrix_tms (tms: list term) (tys: list vty) (P: pat_matrix)
+  (Hty: Forall2 (term_has_type gamma) tms tys)
+  (Hp: pat_matrix_typed tys P) : option (gen_ret pd vt b ret_ty) :=
+  matches_matrix tys (terms_to_hlist tms tys Hty) P Hp.
 
 End MultipleMatchSemantics.
 
+(*Prove the key intermediate results for the S and D matrices.
+  First, we give nicer definitions*)
+
+Definition spec(P: pat_matrix) (c: funsym) : pat_matrix :=
+  Pattern.filter_map (fun x =>
+      let ps := fst x in
+      let a := snd x in
+      match ps with
+      | p :: ps =>
+        match p with
+        | Pwild => Some (repeat Pwild (length (s_args c)) ++ ps, a)
+        | Pconstr fs tys pats =>
+            if funsym_eqb fs c then Some (rev pats ++ ps, a) else None
+        | _ => None
+        end
+      | _ => None
+      end
+) P.
+
+Definition default(P: pat_matrix) : pat_matrix :=
+  Pattern.filter_map (fun x =>
+    match (fst x) with
+    | Pwild :: ps => Some (ps, snd x)
+    | _ => None
+    end ) P.
+
+(*(TODO: prove simplify later)*)
+
+(*The specifications: let ts = t :: tl. By typing, know [[t]] = [[c]](al)
+  1. If c is in first column of P, then [[match((rev al) ++ [[tl]], S(P, c))]] = 
+    [[match(ts, P)]] 
+  2. If c is not in the first column of P, then [[match(tl, D(P, c))]] = [[match(ts, P)]]*)
+
+
+
+(*A predicate that says "term t has semantic meaning c(al), where c is a constructor
+  in ADT a in mutual m"*)
+Definition tm_semantic_constr (t: term) {m: mut_adt} (m_in : mut_in_ctx m gamma)
+  {a: alg_datatype} (a_in: adt_in_mut a m) {c: funsym} (c_in: constr_in_adt c a) 
+  {args: list vty} (args_len: length args = length (m_params m))
+  (Hty: term_has_type gamma t (vty_cons (adt_name a) args))
+  (al: arg_list (domain (dom_aux pd)) (sym_sigma_args c (map (v_subst vt) args)))
+   : Prop :=
+  (*[[t]] =*)
+  term_rep gamma_valid pd vt pf v t _ Hty = dom_cast (dom_aux pd) (*Need 2 casts*)
+    (eq_sym (v_subst_cons (adt_name a) args)) 
+  (scast 
+    (eq_sym (adts pd m (map (v_subst vt) args) a a_in))
+  (* [[c]](al)*)
+  (constr_rep gamma_valid m m_in 
+    (map (v_subst vt) args) (eq_trans (map_length _ _) args_len) (dom_aux pd) a a_in 
+      c c_in (adts pd m (map (v_subst vt) args)) 
+         al)).
+
+(*TODO: move*)
+Equations hlist_app {A: Type} (f: A -> Type) (l1 l2: list A) (h1: hlist f l1) (h2: hlist f l2):
+  hlist f (l1 ++ l2) :=
+  hlist_app f nil l2 h1 h2 := h2;
+  hlist_app f (x :: l1) l2 (HL_cons _ a1 htl) h2 := HL_cons _ _ _ a1 (hlist_app f l1 l2 htl h2).
+
+Equations hlist_rev {A: Type} (f: A -> Type) (l: list A) (h: hlist f l) : hlist f (rev l) :=
+  hlist_rev f nil h := h;
+  hlist_rev f (x :: t) (HL_cons _ a1 htl) := hlist_app f (rev t) [x] (hlist_rev f t htl) 
+    (HL_cons _ _ _ a1 (HL_nil _)).
+
+(*Is there a better way to do this without all the casting, etc*)
+
+(*An easy cast, just a bunch of maps, revs, and apps together*)
+Lemma spec_prop_cast params sargs args tys : (map (v_subst vt)
+  (rev
+  (sorts_to_tys
+  (ty_subst_list_s params (map (v_subst vt) args)
+  sargs)) ++
+tys)) = (rev (ty_subst_list_s params  (map (v_subst vt) args) sargs)) ++
+map (v_subst vt) tys.
+Proof.
+  unfold sorts_to_tys, ty_subst_list_s. rewrite !map_map, !map_app, !map_rev, !map_map.
+  f_equal. f_equal. apply map_ext. intros. rewrite <- subst_sort_eq; reflexivity.
+Qed. 
+
+Set Bullet Behavior "Strict Subproofs".
+Lemma spec_prop 
+  (*Info about first term*)
+  (t: term) {m: mut_adt} (m_in : mut_in_ctx m gamma)
+  {a: alg_datatype} (a_in: adt_in_mut a m) {c: funsym} (c_in: constr_in_adt c a) 
+  {args: list vty} (args_len: length args = length (m_params m))
+  (Hty: term_has_type gamma t (vty_cons (adt_name a) args))
+  (al1: arg_list (domain (dom_aux pd)) (sym_sigma_args c (map (v_subst vt) args)))
+  (Ht: tm_semantic_constr t m_in a_in c_in args_len Hty al1)
+  (*Info about rest of terms*)
+  (ts: list term) (tys: list vty) (al2: arg_list (domain (dom_aux pd)) (map (v_subst vt) tys))
+  (Htsty: Forall2 (term_has_type gamma) (t :: ts) (vty_cons (adt_name a) args :: tys)) (*duplicate proof for irrelevance*)
+  (*Info about pattern matrix*)
+  (P: pat_matrix) (Hpsimp: simplified P) (*(Hc: constr_at_head_ex c P)*) (*TODO: don't think we need - SEEE*)
+  (Htyp: pat_matrix_typed (vty_cons (adt_name a) args :: tys) P)
+  (Htyp': pat_matrix_typed (rev (sorts_to_tys (ty_subst_list_s (s_params c) (map (v_subst vt) args) (s_args c))) ++ tys)
+    (spec P c)):
+
+  matches_matrix_tms (t :: ts) (vty_cons (adt_name a) args :: tys) P
+    Htsty Htyp =
+
+  matches_matrix 
+  (*Type list more complicated: args of c + rest*)
+  (rev (sorts_to_tys (ty_subst_list_s (s_params c) (map (v_subst vt) args) (s_args c))) ++ tys)
+    (cast_arg_list (eq_sym (spec_prop_cast (s_params c) (s_args c) args tys))
+   (hlist_app _ _ _ (hlist_rev _ _ al1) (terms_to_hlist ts tys (Forall2_inv_tail Htsty))))
+    (spec P c) Htyp'.
+Proof.
+  unfold matches_matrix_tms.
+  generalize dependent (eq_sym (spec_prop_cast (s_params c) (s_args c) args tys)).
+  generalize dependent (Forall2_inv_tail Htsty).
+  revert Htsty Htyp Htyp'.
+  unfold matches_matrix_tms. (*TODO: get [matches_matrix_elim] to work?*)
+  induction P as [| rhd rtl].
+  - intros. simpl. rewrite !matches_matrix_equation_1. reflexivity.
+  - intros. simpl. rewrite !matches_matrix_equation_2.
+    destruct rhd as [ps a1]; simpl.
+    (*Case on patterns*)
+    destruct ps as [| phd ptl].
+    + (*TODO: prove that we cannot have nil row in matrix if well-typed*) admit.
+    + destruct phd as [| f' params tms | | |]; try discriminate.
+      * (*Interesting case: Pconstr*)
+        revert Htyp'. simpl.
+        destruct (funsym_eqb_spec f' c); subst; simpl; intros.
+        (*TODO: need to decompose [matches_matrix] for app (matches_matrix (tys1 ++ tys2) (hlist_app h1 h2)
+          = matches_matrix tys1 h1 && matches_matrix tys2 h2 (assuming lengths are correct and && = option bind)
+          then prove that the first one is equal to this [matches_row]
+          )*)
+        -- rewrite matches_matrix_equation_2. simpl.
+        (*Above is wrong - need to just decompose [matches_row] in way described above
+          and then prove that [match_val_single] in constr case (assuming we know constr matches)
+          is equal to [matches_row] for that given arg list - result follows from this*)
+
+        2: {
+
+        }
+        (*TODO: prove that match_val_single, in constr_case (if equal) is equal to
+          matches_row*)
+
+
+      * try discriminate. (*Pvar case*) rewrite matches_row_equation_4.
+
+    (*Really, what we want to prove:
+      Suppose that (t :: ts) matches row r*)
+
+
+    rewrite terms_to_hlist_equation_4.
+    destruct ps as [| phd ptl].
+    + (*TODO: prove that we cannot have nil row in matrix if well-typed*) admit.
+    + rewrite matches_row_equation_4.
+      (*Think we need a different lemma*)
+      destruct phd.
+      * simpl.
+      unfold match_val_single at 1.
+      (*Core of the proof: *)
+    
+    
+   rewrite (matches_row_equation_4 (vty_cons (adt_name a) args) tys
+      (HL_cons (domain (dom_aux pd))
+  (v_subst vt (vty_cons (adt_name a) args))
+  (map (v_subst vt) tys)
+  (term_rep gamma_valid pd vt pf v t
+  (vty_cons (adt_name a) args) (Forall2_inv_head Htsty))
+  (terms_to_hlist ts tys (Forall2_inv_tail Htsty)))).
+    (*Probably need: if matches_row *)
+
+    Check matches_row_equation_4.
+    rewrite matches_row_equation_4.
+
+    simpl in Hc. unfold constr_at_head in Hc.
+
+
+  
+   unfold matches_matrix_tms.
+    Search matches_matrix.
+    simpl.
+    Print matches_matrix.
+
+
+
+  generalize dependent Hty. Htysty.
+
+
+
+has type
+"hlist (domain (dom_aux pd))
+  (rev (sym_sigma_args c (map (v_subst vt) args)) ++
+map (v_subst vt) tys)"
+while it is expected to have type
+"arg_list (domain (dom_aux pd))
+  (map (v_subst vt)
+  (sorts_to_tys
+  (ty_subst_list_s (s_params c) (map (v_subst vt) args)
+  (s_args c)) ++
+tys))".
+
+
+
+
+Definition matches_matrix_tms (tms: list term) (tys: list vty) (P: pat_matrix)
+  (Hty: Forall2 (term_has_type gamma) tms tys)
+  (Hp: pat_matrix_typed tys P) : option (gen_ret pd vt b ret_ty) :=
+  matches_matrix tys (terms_to_hlist tms tys Hty) P Hp.
+
+
+
+
+(tl: list term) (c: funsym) (ty1: vty) (tys1: list vty) 
+  (al: arg_list (domain (dom_aux pd)) (map (v_subst vt) tys1))
+  (P: pat_matrix)
+  (Hsimp: simplified P)
+  (Hc: constr_at_head_ex c P) Hty1 Htyp:
+  
+  matches_matrix (terms_to_hlist (t :: tl) (ty1 :: tys1) Hty1) P Htyp =
+  matches_matrix (hlist_app (hlist_rev al) 
+
+
+Lemma default_prop
+
+
+
+
+(tys: list vty) 
+  (al: arg_list (domain (dom_aux pd)) (map (v_subst vt) tys))
+  (p: pat_matrix)
+  (Hty: pat_matrix_typed tys p)
